pulse/src/syntax_extension/PulseSyntaxExtension.Sugar.fst
@@ -180,6 +180,7 @@ and fn_defn = {
   ascription:either computation_type (option A.term);
   measure:option A.term; // with binders in scope
   body:either stmt lambda;
+  decorations:list A.decoration;  
   range:rng
 }
 
@@ -193,6 +194,7 @@ type fn_decl = {
   id:ident;
   binders:binders;
   ascription:either computation_type (option A.term); (* always Inl for now *)
+  decorations:list A.decoration;
   range:rng
 }
 
@@ -485,7 +487,11 @@ let mk_comp tag precondition return_name return_type postcondition opens range =
      opens;
      range
   }
-
+let add_decorations d ds =
+  match d with
+  | FnDefn f -> FnDefn { f with decorations=ds @ f.decorations }
+  | FnDecl f -> FnDecl { f with decorations=ds @ f.decorations }
+  
 // let mk_slprop_exists binders body = SLPropExists { binders; body }
 let mk_expr e = Expr { e }
 let mk_assignment id value = Assignment { lhs=id; value }
@@ -498,8 +504,12 @@ let mk_while guard id invariant body = While { guard; id; invariant; body }
 let mk_intro slprop witnesses = Introduce { slprop; witnesses }
 let mk_sequence s1 s2 = Sequence { s1; s2 }
 let mk_stmt s range = { s; range }
-let mk_fn_defn id is_rec binders ascription measure body range : fn_defn = { id; is_rec; binders; ascription; measure; body; range }
-let mk_fn_decl id binders ascription range : fn_decl = { id; binders; ascription; range }
+let mk_fn_defn id is_rec binders ascription measure body decorations range
+: fn_defn
+= { id; is_rec; binders; ascription; measure; body; decorations; range }
+let mk_fn_decl id binders ascription decorations range
+: fn_decl
+= { id; binders; ascription; decorations; range }
 let mk_open lid = Open lid
 let mk_par p1 p2 q1 q2 b1 b2 = Parallel { p1; p2; q1; q2; b1; b2 }
 let mk_proof_hint_with_binders ht bs =  ProofHintWithBinders { hint_type=ht; binders=bs }
